coq/apex.v
@@ -1,0 +1,53 @@
+Require Import Ssreflect.ssreflect Ssreflect.ssrbool Ssreflect.ssrnat.
+Require Import Ssreflect.eqtype Ssreflect.ssrfun Ssreflect.seq.
+Require Import MathComp.path.
+Require Import Eqdep pred idynamic ordtype pcm finmap unionmap heap coding. 
+Require Import hgraphs logs.
+Set Implicit Arguments.
+Unset Strict Implicit.
+Unset Printing Implicit Defensive. 
+
+Section ApexAlgo.
+
+(* Initial graph an heap *)
+Variables (h0 : heap) (g0: graph h0).
+
+(* A good log p wrt. initial heap h0 *)
+Variables (p : log) (pf: goodLog (keys_of h0) p) (upf : uniq p).
+
+(* Final heap and graph *)
+Variables (h : heap) (g: graph h).
+Variable (epf : executeLog g0 p = Some (ExRes g)).
+
+(* Dereferencing an object field *)
+Notation "o '#' f" := (nth null (fields g o) f)
+  (at level 43, left associativity).
+
+(******************************************************************)
+(*    Apex procedure for exposing reachable objects in the graph  *)
+(******************************************************************)
+
+Eval compute in let lst := [:: 1; 2; 3] in take (index 1 lst) lst.
+
+
+(* 
+
+To simplify the implementation, we ensure that all entries in the log
+are unique (see the assumption 'upf'). Therefore, the prefix 'prepi'
+is unambiguously defined for each entry in the log, and is computed by
+an entry itself, not a specific index.
+*)
+
+Definition expose_apex := 
+  [seq let o := (source pi) in
+       let f := (fld pi)    in 
+       o#f | pi <- p &
+             let o     := (source pi)           in
+             let f     := (fld pi)              in   
+             let k     := (kind pi)             in   
+             let prepi := (take (index pi p) p) in
+             (kindMA k) && ((o, f) \in wavefront prepi)].
+
+
+
+End ApexAlgo.
